Fixed bug in gc config.h; correct some size-bound proofs
1. OCaml's config.h was relying on auto-generated header file m.h
  to define SIZEOF_PTR and SIZEOF_LONG, but we were not providing
  that file;  now we use CompCert ccomp to generate it correctly.

2. Define MAX_SPACES correctly, document it better in a comment,
  fix some Coq proofs about bounds related (indirectly) to MAX_SPACES.
  This is needed to prove that certain pointer-arithmetic C code
  (which uses signed integer divide) is correct.

CertiGC/GC Source/config.h
@@ -16,6 +16,11 @@
 #ifndef CONFIG_H
 #define CONFIG_H
 
+#if SIZEOF_PTR > 0
+#else
+#error "Oops! SIZEOF_PTR is not defined"
+#endif
+
 #if SIZEOF_PTR == SIZEOF_LONG
 /* Standard models: ILP32 or I32LP64 */
 typedef long intnat;
