CertiGC/GC Source/printm.c
@@ -1,0 +1,6 @@
+#include <stdio.h>
+int main (void) {
+  printf("#define SIZEOF_PTR %d\n#define SIZEOF_LONG %d\n#define SIZEOF_INT %d\n",
+	 sizeof(void*), sizeof(long), sizeof(int));
+  return 0;
+}
