Makefile
@@ -235,15 +235,21 @@ VST_CRITICAL_FILES = \
 
 clightgen:
 	cp CertiGC/'GC Source'/{config.h,gc.h,mem.h,values.h,gc.c} CertiGC
+	cd CertiGC/'GC Source'; `dirname $(CLIGHTGEN)`/ccomp printm.c -o printm
+	CertiGC/'GC Source'/printm >CertiGC/m.h
 	$(CLIGHTGEN) -DCOMPCERT -normalize -isystem . $(C_FILES)
 
 clightgen64:
 	cp CertiGC/'GC Source'/{config.h,gc.h,mem.h,values.h,gc.c} CertiGC
+	cd CertiGC/'GC Source'; `dirname $(CLIGHTGEN64)`/ccomp printm.c -o printm
+	CertiGC/'GC Source'/printm >CertiGC/m.h
 	$(CLIGHTGEN64) -DCOMPCERT -normalize -isystem . $(C_FILES)
 	$(foreach x,$(C_FILES:%.c=%), mv $(x).v $(x)64.v; )
 
 clightgen32:
 	cp CertiGC/'GC Source'/{config.h,gc.h,mem.h,values.h,gc.c} CertiGC
+	cd CertiGC/'GC Source'; `dirname $(CLIGHTGEN32)`/ccomp printm.c -o printm
+	CertiGC/'GC Source'/printm >CertiGC/m.h
 	$(CLIGHTGEN32) -DCOMPCERT -normalize -isystem . $(C_FILES)
 	$(foreach x,$(C_FILES:%.c=%), mv $(x).v $(x)32.v; )
 
